compcert/lib/Decidableplus.v
@@ -19,55 +19,8 @@
   of Coq 8.5 with more instances of decidable properties, including
   universal and existential quantification over finite types. *)
 
-(** Temporarily and for compatibility with Coq 8.4, this file includes
-  a copy of the relevant definitions from the Coq 8.5 [DecidableClass]
-  library.  This library is copyright INRIA. *)
-
+Require Export DecidableClass.
 Require Import Coqlib.
-
-Class Decidable (P : Prop) := {
-  Decidable_witness : bool;
-  Decidable_spec : Decidable_witness = true <-> P
-}.
-
-Lemma Decidable_sound : forall P (H : Decidable P),
-  Decidable_witness = true -> P.
-Proof.
-  intros. rewrite <- Decidable_spec. auto.
-Qed.
-
-Lemma Decidable_complete : forall P (H : Decidable P),
-  P -> Decidable_witness = true.
-Proof.
-  intros. rewrite Decidable_spec. auto.
-Qed.
-
-Lemma Decidable_sound_alt : forall P (H : Decidable P),
-   ~ P -> Decidable_witness = false.
-Proof.
-  intros. destruct Decidable_witness eqn:E; auto. elim H0. eapply Decidable_sound; eauto.
-Qed.
-
-Lemma Decidable_complete_alt : forall P (H : Decidable P),
-  Decidable_witness = false -> ~ P.
-Proof.
-  intros; red; intros. rewrite (Decidable_complete P H) in H0 by auto. discriminate.
-Qed.
-
-Definition decide P {H : Decidable P} := Decidable_witness (Decidable:=H).
-
-Ltac _decide_ P H :=
-  let b := fresh "b" in
-  set (b := decide P) in *;
-  assert (H : decide P = b) by reflexivity;
-  clearbody b;
-  destruct b; [apply Decidable_sound in H|apply Decidable_complete_alt in H].
-
-Tactic Notation "decide" constr(P) "as" ident(H) :=
-  _decide_ P H.
-
-Tactic Notation "decide" constr(P) :=
-  let H := fresh "H" in _decide_ P H.
 
 Ltac decide_goal := eapply Decidable_sound; reflexivity.
 
@@ -77,14 +30,14 @@ Program Instance Decidable_not (P: Prop) (dP: Decidable P) : Decidable (~ P) := 
   Decidable_witness := negb (@Decidable_witness P dP)
 }.
 Next Obligation.
-  rewrite negb_true_iff. split. apply Decidable_complete_alt. apply Decidable_sound_alt. 
+  rewrite negb_true_iff. split. apply Decidable_complete_alt. apply Decidable_sound_alt.
 Qed.
 
 Program Instance Decidable_equiv (P Q: Prop) (dP: Decidable P) (dQ: Decidable Q) : Decidable (P <-> Q) := {
   Decidable_witness := Bool.eqb (@Decidable_witness P dP) (@Decidable_witness Q dQ)
 }.
 Next Obligation.
-  rewrite eqb_true_iff. 
+  rewrite eqb_true_iff.
   split; intros.
   split; intros; eapply Decidable_sound; [rewrite <- H | rewrite H]; eapply Decidable_complete; eauto.
   destruct (@Decidable_witness Q dQ) eqn:D.
@@ -112,7 +65,7 @@ Program Instance Decidable_implies (P Q: Prop) (dP: Decidable P) (dQ: Decidable 
 Next Obligation.
   split.
 - intros. rewrite Decidable_complete in H by auto. eapply Decidable_sound; eauto.
-- intros. destruct (@Decidable_witness P dP) eqn:WP; auto. 
+- intros. destruct (@Decidable_witness P dP) eqn:WP; auto.
   eapply Decidable_complete. apply H. eapply Decidable_sound; eauto.
 Qed.
 
@@ -122,7 +75,7 @@ Program Definition Decidable_eq {A: Type} (eqdec: forall (x y: A), {x=y} + {x<>y
   Decidable_witness := proj_sumbool (eqdec x y)
 |}.
 Next Obligation.
-  split; intros. InvBooleans. auto. subst y. apply dec_eq_true. 
+  split; intros. InvBooleans. auto. subst y. apply dec_eq_true.
 Qed.
 
 Program Instance Decidable_eq_bool : forall (x y : bool), Decidable (eq x y) := {
@@ -133,10 +86,10 @@ Next Obligation.
 Qed.
 
 Program Instance Decidable_eq_nat : forall (x y : nat), Decidable (eq x y) := {
-  Decidable_witness := beq_nat x y
+  Decidable_witness := Nat.eqb x y
 }.
 Next Obligation.
-  apply beq_nat_true_iff.
+  apply Nat.eqb_eq.
 Qed.
 
 Program Instance Decidable_eq_positive : forall (x y : positive), Decidable (eq x y) := {
@@ -159,19 +112,47 @@ Program Instance Decidable_le_Z : forall (x y: Z), Decidable (x <= y) := {
   Decidable_witness := Z.leb x y
 }.
 Next Obligation.
-  apply Z.leb_le. 
+  apply Z.leb_le.
 Qed.
 
 Program Instance Decidable_lt_Z : forall (x y: Z), Decidable (x < y) := {
   Decidable_witness := Z.ltb x y
 }.
 Next Obligation.
-  apply Z.ltb_lt. 
+  apply Z.ltb_lt.
+Qed.
+
+Program Instance Decidable_ge_Z : forall (x y: Z), Decidable (x >= y) := {
+  Decidable_witness := Z.geb x y
+}.
+Next Obligation.
+  rewrite Z.geb_le. intuition omega.
+Qed.
+
+Program Instance Decidable_gt_Z : forall (x y: Z), Decidable (x > y) := {
+  Decidable_witness := Z.gtb x y
+}.
+Next Obligation.
+  rewrite Z.gtb_lt. intuition omega.
+Qed.
+
+Program Instance Decidable_divides : forall (x y: Z), Decidable (x | y) := {
+  Decidable_witness := Z.eqb y ((y / x) * x)%Z
+}.
+Next Obligation.
+  split.
+  intros. apply Z.eqb_eq in H. exists (y / x). auto.
+  intros [k EQ]. apply Z.eqb_eq.
+  destruct (Z.eq_dec x 0).
+  subst x. rewrite Z.mul_0_r in EQ. subst y. reflexivity.
+  assert (k = y / x).
+  { apply Zdiv_unique_full with 0. red; omega. rewrite EQ; ring. }
+  congruence.
 Qed.
 
 (** Deciding properties over lists *)
 
-Program Instance Decidable_forall_in_list : 
+Program Instance Decidable_forall_in_list :
       forall (A: Type) (l: list A) (P: A -> Prop) (dP: forall x:A, Decidable (P x)),
       Decidable (forall x:A, In x l -> P x) := {
   Decidable_witness := List.forallb (fun x => @Decidable_witness (P x) (dP x)) l
@@ -179,10 +160,10 @@ Program Instance Decidable_forall_in_list :
 Next Obligation.
   rewrite List.forallb_forall. split; intros.
 - eapply Decidable_sound; eauto.
-- eapply Decidable_complete; eauto. 
+- eapply Decidable_complete; eauto.
 Qed.
 
-Program Instance Decidable_exists_in_list : 
+Program Instance Decidable_exists_in_list :
       forall (A: Type) (l: list A) (P: A -> Prop) (dP: forall x:A, Decidable (P x)),
       Decidable (exists x:A, In x l /\ P x) := {
   Decidable_witness := List.existsb (fun x => @Decidable_witness (P x) (dP x)) l
@@ -207,8 +188,8 @@ Program Instance Decidable_forall : forall (T: Type) (fT: Finite T) (P: T -> Pro
 }.
 Next Obligation.
   rewrite List.forallb_forall. split; intros.
-- eapply Decidable_sound; eauto. apply H. apply Finite_elements_spec. 
-- eapply Decidable_complete; eauto. 
+- eapply Decidable_sound; eauto. apply H. apply Finite_elements_spec.
+- eapply Decidable_complete; eauto.
 Qed.
 
 Program Instance Decidable_exists : forall (T: Type) (fT: Finite T) (P: T -> Prop) (dP: forall x:T, Decidable (P x)), Decidable (exists x, P x) := {
@@ -217,7 +198,7 @@ Program Instance Decidable_exists : forall (T: Type) (fT: Finite T) (P: T -> Pro
 Next Obligation.
   rewrite List.existsb_exists. split.
 - intros (x & A & B). exists x. eapply Decidable_sound; eauto.
-- intros (x & A). exists x; split. eapply Finite_elements_spec. eapply Decidable_complete; eauto. 
+- intros (x & A). exists x; split. eapply Finite_elements_spec. eapply Decidable_complete; eauto.
 Qed.
 
 (** Some examples of finite types. *)
