veric/Clight_sim.v
@@ -1,6 +1,6 @@
 Require Import VST.sepcomp.mem_lemmas.
-Require Import VST.sepcomp.semantics.
-Require Import VST.sepcomp.semantics_lemmas.
+Require Import VST.concurrency.core_semantics.
+Require Import VST.concurrency.memsem_lemmas.
 Require Import VST.sepcomp.simulations.
 Require Import VST.sepcomp.simulations_lemmas.
 (*Require Import VST.sepcomp.compiler_correctness.*)
